Some monoid theorems

theories/syntax.v
@@ -38,8 +38,9 @@ Local Open Scope monad_scope.
 Local Open Scope string_scope.
 
 Inductive expr : Type :=
-| True
-| False
+| Var : nat -> expr
+| True : expr
+| False : expr
 .
 
 Inductive cmd : Type :=
@@ -56,25 +57,85 @@ Inductive cl : Type :=
 | Atom : cmd -> cl
 .
 
+Inductive weight : Type :=
+| Bool : bool -> weight
+| Unit : weight
+.
+
 Inductive noop : Type -> Type :=
 | tt : noop unit.
 
 Notation computation := (ctree noop B02).
 
-Definition state := nat -> expr.
+Definition state := nat -> weight.
 
-Reserved Notation "[[ C ]]".
+Reserved Notation "[[ c ]]".
+Notation "x <<>> y" := (br2 x y) (at level 80).
+Notation "[0]" := Stuck.
+
+Definition insert (x : nat) (w : weight) (st : state) : state :=
+  fun y => if Nat.eq_dec x y then w else st y.
+
+Definition denote_expr (e : expr) (st: state) : weight :=
+  match e with
+    | Var x => st x
+    | True => Bool true
+    | False => Bool false
+  end.
+
+
+Definition test_weight (w : weight) : bool :=
+  match w with
+    | Bool b => b
+    | Unit => false
+  end.
+
+Definition denote_cmd (c : cmd) (st: state) : computation state :=
+  match c with
+    | assume e => if test_weight (denote_expr e st) then ret st else [0]
+    | assign x e => ret (insert x (denote_expr e st) st)
+  end.
 
 Fixpoint denote (C : cl) (st: state) : computation state :=
   match C with
-  | Zero => Stuck
+  | Zero => [0]
   | One => ret st
   | Seq C1 C2 => [[ C1 ]] st >>= [[ C2 ]]
-  | Branch C1 C2 => br2 ([[ C1 ]] st) ([[ C2 ]] st)
+  | Branch C1 C2 => ([[ C1 ]] st) <<>> ([[ C2 ]] st)
   | Star C' =>
-      iter (fun st' => br2
-                         (st'' <-  [[ C' ]] st' ;; ret (inl st''))
-                         (ret (inr st'))) st
-  | _ => Stuck (* TODO *)
+      iter (fun st' => (st'' <-  [[ C' ]] st' ;; ret (inl st''))
+                         <<>>
+                       (ret (inr st'))) st
+  | Atom cmd => denote_cmd cmd st
   end
 where "[[ C ]]" := (denote C).
+Notation "x + y" := (Branch x y).
+Notation "x ;;; y" := (Seq x y) (at level 80).
+
+Theorem monoid_identity_l :
+  forall (C : cl) (st: state) , [[ Zero + C ]] st ~ [[ C ]] st.
+Proof.
+  intros.
+  apply br2_stuck_l.
+Qed.
+
+Theorem monoid_identity_r :
+  forall (C : cl) (st: state) , [[ C + Zero ]] st ~ [[ C ]] st.
+Proof.
+  intros.
+  apply br2_stuck_r.
+Qed.
+
+Theorem monoid_commutative :
+    forall (C1 C2 : cl) (st: state) , [[ C1 + C2 ]] st ~ [[ C2 + C1 ]] st.
+Proof.
+  intros.
+  apply br2_commut.
+Qed.
+
+Theorem monoid_respects_bind :
+  forall (C1 C2 K : cl) (st : state), [[ (C1 + C2);;; K ]] st ~ [[ (C1;;; K) + (C2;;; K) ]] st.
+Proof.
+  intros.
+  simpl.
+Admitted.
